dataplane/Examples/Collatz/Collatz_Nop_Invariant.thy
@@ -1,0 +1,27 @@
+theory Collatz_Nop_Invariant
+
+imports
+  Collatz
+  "../../Timely/Tree_Nop_Invariant"
+begin
+
+section ‹The Optimized and Plain Compiled Collatz Programs are Equivalent›
+
+lemma builder_tree_dt:
+  "builder_tree dt"
+  by (auto intro: nop_leaf_ooo_input_op nop_leaf_concat_op nop_leaf_tmap_op
+      nop_leaf_branch_op nop_leaf_increment_op)
+
+lemma distinct_tree_ids_dt:
+  "distinct (fst (tree_ids (0 :: 5) dt))"
+  by simp
+
+theorem compiled_collatz_wbisim:
+  "compiled ≈ compile_dataflow (λ _. []) dt"
+  by (rule compile_dataflow_opt_wbisim_generic[OF builder_tree_dt distinct_tree_ids_dt])
+
+theorem compiled_collatz_wtraces:
+  "compiled ≡⇩t compile_dataflow (λ _. []) dt"
+  by (rule wbisim_wtraces[OF compiled_collatz_wbisim])
+
+end
