dataplane/Examples/Label_Propagation/Label_Propagation_Nop_Invariant.thy
@@ -1,0 +1,31 @@
+theory Label_Propagation_Nop_Invariant
+
+imports
+  Label_Propagation_op_Correctness_Extras
+  "../../Timely/Tree_Nop_Invariant"
+begin
+
+section ‹The Optimized and Plain Compiled Label Propagation Programs are Equivalent›
+
+lemma builder_tree_G:
+  "builder_tree (G inp_state label_state incr_state)"
+  by (auto intro: nop_leaf_ooo_input_op nop_leaf_label_propagation_op
+      nop_leaf_increment_op)
+
+lemma distinct_tree_ids_G:
+  "distinct (fst (tree_ids (0 :: 3) (G inp_state label_state incr_state)))"
+  by simp
+
+theorem compiled_label_propagation_wbisim:
+  "compiled inp ≈ compile_dataflow (λ _. [])
+     (G (initial_state_input inp) initial_state_label_prop
+        (initial_state_increment (MyPair 0 1)))"
+  by (rule compile_dataflow_opt_wbisim_generic[OF builder_tree_G distinct_tree_ids_G])
+
+theorem compiled_label_propagation_wtraces:
+  "compiled inp ≡⇩t compile_dataflow (λ _. [])
+     (G (initial_state_input inp) initial_state_label_prop
+        (initial_state_increment (MyPair 0 1)))"
+  by (rule wbisim_wtraces[OF compiled_label_propagation_wbisim])
+
+end
